backend/Cminor.v
@@ -242,6 +242,13 @@ Inductive state: Type :=
              (m: mem),                  (**r memory state *)
       state.
 
+Definition Cminor_get_mem (s:state):=
+  match s with
+  | State _ _ _ _ _ m => m
+  | Callstate _ _ _ m => m
+  | Returnstate _ _ m => m
+  end.
+
 (*NEW*)Inductive cstate: Type :=
   | CState:                      (**r Execution within a function *)
       forall (f: function)              (**r currently executing function  *)
