backend/Mach.v
@@ -267,7 +267,14 @@ Inductive state: Type :=
       forall (stack: list stackframe)  (**r call stack *)
              (rs: regset)              (**r register state *)
              (m: mem),                 (**r memory state *)
-      state.
+        state.
+
+Definition Mach_get_mem (s:state):=
+  match s with
+  | State _ _ _ _ _ m => m
+  | Callstate _ _ _ m => m
+  | Returnstate _ _ m => m
+  end.
 
 Definition parent_sp (s: list stackframe) : val :=
   match s with
